some progress; find the right function

src/sort'.lean
@@ -1,24 +1,143 @@
 import data.finset
+import tactic.linarith
 
 section examples
 
 variables {ι : Type*} [linear_order ι] [is_well_order ι ((≤) : ι → ι → Prop)]
 
-def sort' (σ : finset ι) : fin σ.card → σ := λ n, 
-{ val := (finset.sort ((≤) : ι → ι → Prop) σ).nth_le n.1 $ (finset.length_sort (≤) : _ = σ.card).symm ▸ n.2,
-  property := (finset.mem_sort (≤)).mp $ list.nth_le_mem _ _ _ }
+namespace finset
 
-lemma sort'_monotone (σ : finset ι) : monotone (sort' σ) := λ x y h, 
-list.sorted.rel_nth_le_of_le (finset.sort_sorted ((≤) : ι → ι → Prop) σ) 
-    (by { rw finset.length_sort, exact x.2 } : x.val < (finset.sort (≤) σ).length) 
-    (by { rw finset.length_sort, exact y.2 } : y.val < (finset.sort (≤) σ).length) h
+def erase_order_emb_of_fin (s : finset ι) {k : ℕ} (h : s.card = k) (m : fin k) :
+  fin k.pred ↪o ι :=
+{ to_fun := λ n, 
+    if (n.1 < m.1) 
+    then s.order_emb_of_fin h ⟨n.1, lt_trans n.2 $ nat.pred_lt $ λ r, by rw r at m; exact fin_zero_elim m⟩ 
+    else s.order_emb_of_fin h ⟨n.1.succ, by { convert nat.succ_lt_succ n.2, rw nat.succ_pred_eq_of_pos, apply nat.pos_of_ne_zero (λ r, _), rw r at m, exact fin_zero_elim m } ⟩,
+  inj' := λ x y H, begin
+    dsimp only at H,
+    split_ifs at H with hx hy;
+    have := (s.order_emb_of_fin h).inj' H;
+    rw subtype.ext_iff_val at this ⊢,
+    { exact this, },
+    { rw this at *,
+      exfalso,
+      apply hy,
+      exact lt_trans (lt_add_one _) hx, },
+    { rw ← this at *,
+      exfalso,
+      apply hx,
+      exact lt_trans (lt_add_one _) (by assumption) },
+    { apply_fun nat.succ using nat.succ_injective,
+      exact this },
+  end,
+  map_rel_iff' := λ a b, begin
+    split,
+    { intro H,
+      simp only [function.embedding.coe_fn_mk] at H,
+      split_ifs at H with h1 h2 h3,
+      { rw order_embedding.le_iff_le (s.order_emb_of_fin h) at H,
+        convert H },
+      { rw order_embedding.le_iff_le (s.order_emb_of_fin h) at H,
+        change a.1 ≤ b.1.succ at H,
+        change a.1 ≤ b.1,
+        linarith },
+      { rw order_embedding.le_iff_le (s.order_emb_of_fin h) at H,
+        change a.1.succ ≤ b.1 at H,
+        change a.1 ≤ b.1,
+        exfalso,
+        apply h1,
+        transitivity a.1.succ,
+        { exact lt_add_one _ },
+        { exact lt_of_le_of_lt H h3 } },
+      { rw order_embedding.le_iff_le (s.order_emb_of_fin h) at H,
+        change a.1.succ ≤ b.1.succ at H,
+        rw nat.succ_le_succ_iff at H,
+        convert H, } },
+    { intro H,
+      change a.1 ≤ b.1 at H,
+      simp only [function.embedding.coe_fn_mk],
+      split_ifs with h1 h2 h3;
+      rw order_embedding.le_iff_le (s.order_emb_of_fin h),
+      { change a.1 ≤ b.1,
+        exact H },
+      { change a.1 ≤ b.1.succ,
+        transitivity b.1,
+        { exact H },
+        { exact le_of_lt (lt_add_one _) } },
+      { change a.1.succ ≤ b.1,
+        contrapose! h1,
+        rw nat.lt_succ_iff_lt_or_eq at h1,
+        cases h1,
+        { linarith },
+        { rwa h1 at h3 }, },
+      { change a.1.succ ≤ b.1.succ,
+        rwa nat.succ_le_succ_iff } }
+  end }
 
-lemma sort'_strict_mono (σ : finset ι) : strict_mono (sort' σ) := λ x y h, 
-list.sorted.rel_nth_le_of_lt (finset.sort_sorted_lt σ) _ _ h
+example (s : finset ι) {k : ℕ} (h : s.card = k) (m : fin k) : true :=
+begin
+  have := @finset.order_emb_of_fin_unique _ _ (s.erase (s.order_emb_of_fin h m)) k.pred _
+    (s.erase_order_emb_of_fin h m) _ _,
+  
+  trivial;
+  sorry,
+end
+-- def sort' (σ : finset ι) : fin σ.card → ι := 
+-- λ n, (finset.sort ((≤) : ι → ι → Prop) σ).nth_le n.1 $ (finset.length_sort (≤) : _ = σ.card).symm ▸ n.2
+-- -- { val := (finset.sort ((≤) : ι → ι → Prop) σ).nth_le n.1 $ (finset.length_sort (≤) : _ = σ.card).symm ▸ n.2,
+-- --   property := (finset.mem_sort (≤)).mp $ list.nth_le_mem _ _ _ }
 
-lemma sort'_injective (σ : finset ι) : function.injective (sort' σ) :=
-strict_mono.injective $ sort'_strict_mono _
+-- lemma sort'_mem (σ : finset ι) (m : fin σ.card) :
+--   (σ.sort' m) ∈ σ := 
+-- (finset.mem_sort (≤)).mp $ list.nth_le_mem _ _ _
 
-noncomputable lemma sort'_erase (σ : finset ι) : sorry := sorry
+-- lemma sort'_monotone (σ : finset ι) : monotone (sort' σ) := λ x y h, 
+-- list.sorted.rel_nth_le_of_le (finset.sort_sorted ((≤) : ι → ι → Prop) σ) 
+--     (by { rw finset.length_sort, exact x.2 } : x.val < (finset.sort (≤) σ).length) 
+--     (by { rw finset.length_sort, exact y.2 } : y.val < (finset.sort (≤) σ).length) h
+
+-- lemma sort'_strict_mono (σ : finset ι) : strict_mono (sort' σ) := λ x y h, 
+-- list.sorted.rel_nth_le_of_lt (finset.sort_sorted_lt σ) _ _ h
+
+-- lemma sort'_injective (σ : finset ι) : function.injective (sort' σ) :=
+-- strict_mono.injective $ sort'_strict_mono _
+
+-- def erase_nth (σ : finset ι) (m : fin σ.card) : finset ι :=
+-- σ.erase (sort' σ m)
+
+-- lemma erase_nth_card (σ : finset ι) (m : fin σ.card) :
+--   (σ.erase_nth m).card = σ.card.pred :=
+-- begin
+--   haveI : decidable_eq ι := classical.dec_eq _,
+--   unfold erase_nth,
+--   convert @finset.card_erase_eq_ite _ σ (σ.sort' m) _,
+--   rw if_pos (σ.sort'_mem m),
+--   exact nat.pred_eq_sub_one _,
+-- end
+
+-- lemma sort'_erase_case1.aux0 (σ : finset ι) (h0 : σ.card = 0) (m1 : fin σ.card) (m2 : fin σ.card.pred)
+--   (h : m1.1 < m2.1) :
+--   ((σ.erase_nth m1).sort' ⟨m2.1, (σ.erase_nth_card m1).symm ▸ m2.2⟩ : ι) = 
+--   (σ.sort' ⟨m2.1.pred, false.elim $ by rw h0 at m1; exact fin_zero_elim m1⟩) := 
+-- false.elim $ by rw h0 at m1; exact fin_zero_elim m1
+
+-- lemma sort'_erase_case1.aux1 (σ : finset ι) (h0 : σ.card = 1) (m1 : fin σ.card) (m2 : fin σ.card.pred) 
+--   (h : m1.1 < m2.1) : 
+--   ((σ.erase_nth m1).sort' ⟨m2.1, (σ.erase_nth_card m1).symm ▸ m2.2⟩ : ι) = 
+--   (σ.sort' ⟨m2.1.pred, false.elim $ by rw h0 at m2; exact fin_zero_elim m2⟩) :=
+-- false.elim $ by rw h0 at m2; exact fin_zero_elim m2
+
+-- lemma sort'_erease_case2.aux2 (σ : finset ι) (h0 : 2 ≤ σ.card) (m1 : fin σ.card) (m2 : fin σ.card.pred) 
+--   (h : m1.1 < m2.1) : 
+--   ((σ.erase_nth m1).sort' ⟨m2.1, (σ.erase_nth_card m1).symm ▸ m2.2⟩ : ι) = 
+--   (σ.sort' ⟨m2.1.pred, lt_trans (nat.pred_lt_pred (λ r, nat.not_lt_zero m1.1 (r ▸ h)) 
+--     (lt_of_lt_of_le m2.2 $ le_refl _) : m2.1.pred < σ.card.pred.pred) 
+--     (lt_of_le_of_lt (nat.pred_le _ : σ.card.pred.pred ≤ σ.card.pred) (nat.pred_lt $ λ r, by rw r at m1; exact fin_zero_elim m1))⟩) := 
+-- begin
+--   unfold sort' erase_nth,
+--   sorry
+-- end
+
+end finset
 
 end examples
